Kami/Semantics.v
@@ -227,9 +227,9 @@ Definition evalBinBit n1 n2 n3 (op: BinBitOp n1 n2 n3)
     | Band n => @wand n
     | Bor n => @wor n
     | Bxor n => @wxor n
-    | Sll n m => (fun x y => sll x (wordToNat y))
-    | Srl n m => (fun x y => srl x (wordToNat y))
-    | Sra n m => (fun x y => sra x (wordToNat y))
+    | Sll n m => (fun x y => wlshift x (wordToNat y))
+    | Srl n m => (fun x y => wrshift x (wordToNat y))
+    | Sra n m => (fun x y => wrshifta x (wordToNat y))
     | Concat n1 n2 => fun x y => (combine y x)
   end.
 
